AssocList.v
@@ -1,0 +1,36 @@
+(*
+This file contains useful utilities for dealing with association lists
+ *)
+
+From Coq Require Import Lists.List Unicode.Utf8.
+Import ListNotations.
+
+Module Type WithEq.
+  Parameter t : Type.
+  Parameter eq : t → t → Prop.
+  Parameter eq_dec : ∀ (x x' : t), {eq x x'} + {¬ eq x x'}.
+End WithEq.
+
+Module AssocList (A B : WithEq).
+
+  Definition assoc_list := list (A.t * B.t).
+
+  Definition t := assoc_list.
+
+  Fixpoint lookup (l : assoc_list) (a : A.t) : option B.t :=
+    match l with
+    | [] => None
+    | (a', b') :: l_tail =>
+        if (A.eq_dec a a') then Some b' else
+          lookup l_tail a
+    end.
+
+    
+  Definition contains (l : assoc_list) a b : Prop :=
+    lookup l a = Some b.
+  
+  Definition eq l₁ l₂ : Prop :=
+    ∀ a b, contains l₁ a b ↔ contains l₂ a b.
+
+  Global Notation "[ l ; a ↦ b ]" := ((a, b) :: l).
+End AssocList.
