Noninterference.v
@@ -1,0 +1,31 @@
+From NITraces Require Import Program Traces AssocList Semantics.
+
+From Coq Require Import Lists.List Unicode.Utf8.
+Import ListNotations.
+
+Section MainDefinitions.
+  Context (in_equiv : memory → memory → Prop).
+  Context (out_equiv : memory → memory → Prop).
+
+  Infix "≡ᵢ" := in_equiv (at level 50).
+  Infix "≡ₒ" := out_equiv (at level 50).
+
+  (* classical noninterference *)
+  Definition noninterferent (p : program) :=
+    let e := body p in
+    ∀ mᵢ mᵢ' mₒ mₒ',
+      (mᵢ ≡ᵢ mᵢ') →
+      ⟨e; mᵢ ↓ mₒ⟩ →
+      ⟨e; mᵢ' ↓ mₒ'⟩ →
+      (mₒ ≡ₒ mₒ').
+
+  (* trace noninterference *)
+  Definition trace_noninterference (p : program) (t : trace) :=
+    let e := body p in
+    ∀ mᵢ mᵢ' mₒ mₒ',
+      (mᵢ ≡ᵢ mᵢ') →
+      ⟨e; mᵢ ↓ mₒ; t⟩ →
+      ⟨e; mᵢ' ↓ mₒ'⟩ →
+      (mₒ ≡ₒ mₒ').
+
+End MainDefinitions.
