Semantics.v
@@ -1,0 +1,201 @@
+(*
+The primary contribution of this file is the definition of the stack and heap types,
+which includes the definitions of the _values_ used in them, in service of defining
+the big step operational semantics for our programs from Program.v. Because unequal
+trace, stack, and heap values can be semantically considered equal, the big step
+semantics contains a case for deriving across known semantic equality such as `mem_eq`.
+
+Also of note in this file is the function `eval_branch_in_memory` - it is responsible
+for checking whether a given branch on a given variable in a given memory state
+should be taken in the true or false direction - a key component of our semantics
+
+ *)
+
+From NITraces Require Import Program Traces AssocList.
+
+From Coq Require Import Lists.List Unicode.Utf8.
+Import ListNotations.
+
+(* base values are the core set of values that stack variables can take -
+   modeled as integers *)
+Inductive base_value := BaseValue (n : nat).
+
+(* module-ize *)
+Module BaseValue.
+  Definition t := base_value.
+  Definition eq := @eq t.
+  Definition eq_dec : ∀ (x x' : t), {eq x x'} + {~eq x x'}.
+  Proof.
+    unfold eq.
+    decide equality.
+    apply PeanoNat.Nat.eq_dec.
+  Defined.
+End BaseValue.
+
+(* values themselves are the base values closed over the set of operators -
+   since there are no equalities or other properties of these operators,
+   values are equavalent to syntax trees *)
+Inductive value :=
+| One : base_value → value
+| Composite : value → operator → value → value.
+
+(* notation for lifting base values to values *)
+Notation "⦇ bv ⦈" := (One bv).
+Notation "⦇ v₀ ⊕ [ op ] v₁ ⦈" := (Composite v₀ op v₁).
+
+(* the following definitions provide a non-duplicating append operation
+on lists of base values *)
+
+Definition nodup_val_cons (v : base_value) (lv : list base_value) :=
+  if (List.in_dec BaseValue.eq_dec v lv) then lv else v :: lv.
+
+Fixpoint nodup_val_app (lv₀ lv₁ : list base_value) :=
+  match lv₀ with
+  | [] => lv₁
+  | v :: lv₀_tail => nodup_val_app lv₀_tail (nodup_val_cons v lv₁)
+  end.
+
+Lemma nodup_val_app_sound : ∀ lv₀ lv₁,
+    (NoDup lv₀) → (NoDup lv₁) → (NoDup (nodup_val_app lv₀ lv₁)).
+Admitted.
+
+(* reduce a value to a non-duplicated list of underlying base values *)
+Fixpoint flatten_vals (v : value) : list base_value :=
+  match v with
+  | ⦇ bv ⦈ => [bv]
+  | ⦇ v₀ ⊕[_] v₁ ⦈ => nodup_val_app (flatten_vals v₀) (flatten_vals v₁)
+  end.
+
+(* module-ize *)
+Module Value.
+  Definition t := value.
+  Definition eq := @eq t.
+  Definition eq_dec : ∀ (x x' : t), {eq x x'} + {~eq x x'}.
+  Proof.
+    unfold eq.
+    decide equality.
+    apply BaseValue.eq_dec.
+    apply Op.eq_dec.
+  Defined.
+End Value.
+(* a stack maps stack variables (defined in Program.v) to values *)
+Module Stack := AssocList Var Value.
+
+(* lists of branches are equal if they contain the same elements *)
+Module BranchList.
+  Definition t := list branch.
+  Definition eq lb₁ lb₂ := ∀ b : branch, (In b lb₁) ↔ (In b lb₂).
+  Definition eq_dec : ∀ (x x' : t), {eq x x'} + {~eq x x'}.
+    Admitted.
+End BranchList.
+
+(* a heap maps the base values to their "interpretations" - the
+   interpretation for a base value is the direction that it causes
+   each branch to take if it is inspected in that branch's guard
+   (hence - it is a vector of size equal to the number of branches).
+   The underlying storage for these vectors is sparse - it is a set of
+   their one components.  In the case that multiple values are
+   inspected in a given guard, the xor of the individual components
+   for each value is taken as the value that determines the direction
+   the branch will be taken. *)
+Module Heap := AssocList BaseValue BranchList.
+
+(* memory consists of a stack and a heap *)
+Definition memory : Type := Stack.t * Heap.t.
+
+(* semantic equality for memory states *)
+Definition mem_eq (m₁ m₂ : memory) :=
+  let (σ₁, ρ₁) := m₁ in
+  let (σ₂, ρ₂) := m₂ in
+  Stack.eq σ₁ σ₂ ∧ Heap.eq ρ₁ ρ₂.
+                           
+(* this is VERY important - *)
+
+Lemma branch_eq_dec : ∀ v₀ v₁ : branch, {v₀ = v₁} + {v₀ ≠ v₁}.
+  decide equality.
+  apply PeanoNat.Nat.eq_dec.
+Qed.
+
+(* this function looks up each base_value in the passed list in the passed heap. If all
+lookups succeed, Some is returned with the result of the lookups. Otherwise None is returned *)
+Fixpoint lookup_in_heap (ρ : Heap.t) (lb : list base_value) : option (list (list branch)) :=
+  match lb with
+  | [] => Some []
+  | bv :: lb_tail =>
+      match (Heap.lookup ρ bv, lookup_in_heap ρ lb_tail) with
+      | (Some looked_up_bv, Some looked_up_lb_tail) => Some (looked_up_bv :: looked_up_lb_tail)
+      | _ => None
+      end
+  end.
+
+(* this proposition encodes the fact that the branch `b`, which has as guard variable `x`,
+will take direction `dir` in memory state `m`. This is the most important aspect of our
+semantics. In particular, each base_value that was involved in the computation of `x`
+is looked up in the heap, and the `b`th component of the bitstring found for each
+heap lookup is xor'd together. This ensures each value has influence on the branch
+direction.
+*)
+Definition eval_branch_in_memory (b : branch) (x : variable) (m : memory) (dir : bool) : Prop :=
+  let (σ, ρ) := m in
+  ∃ v, (Stack.contains σ x v) ∧
+         let base_vals := flatten_vals v in
+         match (lookup_in_heap ρ base_vals) with
+         | None => False
+         | Some base_val_bitstrings  =>
+             let project bitstring :=
+               if List.in_dec Branch.eq_dec b bitstring then true else false
+             in
+             (List.fold_right (fun bitstring => xorb (project bitstring))
+                false base_val_bitstrings) = dir
+         end.
+
+
+Definition ε : trace := nil.
+
+Notation "[ l ; a ↦ b ]" := ((a, b) :: l) (at level 50).
+
+Reserved Notation "⟨ e ; m₀ ↓ m₁ ; t ⟩" (at level 50).
+
+Inductive eval_with_trace : expression → memory → memory → trace → Prop :=
+(* the EquivEval constructor generalizes the eval relation across equal arguments *)
+| EquivEval : ∀ e m₀ m₀' m₁ m₁' t t',
+    ⟨e ; m₀ ↓ m₁ ; t⟩ →
+    (mem_eq m₀ m₀') →
+    (mem_eq m₁ m₁') →
+    (Trace.eq t t') →
+    ⟨e; m₀' ↓ m₁' ; t'⟩
+(* the AssignEval constructor evaluates assignments by looking up both operands in the stack,
+and mapping the assigned value in the stack to the syntactically provided operator
+applies to the values of the operands *)
+| AssignEval : ∀ σ ρ x₀ x₁ x₂ v₁ v₂ o,
+    (Stack.contains σ x₁ v₁) →
+    (Stack.contains σ x₂ v₂) →
+    ⟨⦃(x₀) = (x₁) ⊕[o] (x₂)⦄; (σ, ρ) ↓ ([σ ; x₀ ↦ ⦇v₁ ⊕[o] v₂⦈], ρ); ε⟩
+(* the BranchEval rules evaluate branches by checking their guard
+using the eval_branch_in_memory prop, and then sequencing
+the true or false branch to get a new memory state that additionally
+ has the direction of this branch noted in its guard *)                  
+| BranchEvalTrue : ∀ σ ρ σ' ρ' x b e₀ e₁ t,
+    (eval_branch_in_memory b x (σ, ρ) true) →
+    ⟨e₀; (σ, ρ) ↓ (σ', ρ'); t⟩ →
+    ⟨⦃if[b] (x) then {{e₀}} else {{e₁}}⦄; (σ, ρ) ↓ (σ', ρ'); [t; b ↦ true]⟩
+| BranchEvalFalse : ∀ σ ρ σ' ρ' x b e₀ e₁ t,
+    (eval_branch_in_memory b x (σ, ρ) true) →
+    ⟨e₀; (σ, ρ) ↓ (σ', ρ'); t⟩ →
+    ⟨⦃if[b] (x) then {{e₀}} else {{e₁}}⦄; (σ, ρ) ↓ (σ', ρ'); [t; b ↦ true]⟩
+(* the SeqEval rule sequences the evaluation of two expression as expected,
+ only interesting part is that traces get appended*)
+| SeqEval : ∀ m₀ m₁ m₂ e₀ e₁ t₀ t₁,
+    ⟨e₀; m₀ ↓ m₁; t₀⟩ →
+    ⟨e₁; m₁ ↓ m₂; t₁⟩ →
+    ⟨⦃{e₀}; {e₁}⦄; m₀ ↓ m₂; t₀ ++ t₁⟩
+where "⟨ e ; m₀ ↓ m₁ ; t ⟩" := (eval_with_trace e m₀ m₁ t).
+
+(* this is a version of the evaluation relation that discards information about traces *)
+Definition eval (e : expression) (m₀ m₁ : memory) : Prop := ∃ t, ⟨e; m₀ ↓ m₁; t⟩.
+
+Notation "⟨ e ; m₀ ↓ m₁ ⟩" := (eval e m₀ m₁) (at level 50).
+
+(*TODO: write some examples testing the semantics *)
+
+
