Traces.v
@@ -1,0 +1,48 @@
+(*
+The primary contribution of this file is to define the type `trace`
+representing a trace of a program.
+
+The function `program_traces` computes the traces of a program `p`.
+The function `trace_eq` is equality for traces.
+
+*)
+
+From NITraces Require Import Program AssocList.
+
+From Coq Require Import Lists.List Unicode.Utf8.
+Import ListNotations.
+  
+Module Trace := AssocList Branch Bool.
+Definition trace := Trace.t.
+
+(* given a trace `tr` and trace list `trl`, return
+each trace in `trl` with `tr` appended to its front *)
+Fixpoint append_trace (tr : Trace.t) trl :=
+  match trl with
+  | [] => []
+  | tr' :: trl_tail => (tr ++ tr') :: (append_trace tr trl_tail)
+  end.
+
+(* given two trace lists, return the list of traces that can be formed
+by appending a trace from the former with a trace from the latter *)
+Fixpoint append_trace_lists trl₁ trl₂ :=
+  match trl₁ with
+  | [] => []
+  | tr :: trl₁_tail => append_trace tr trl₂ ++ append_trace_lists trl₁_tail trl₂
+  end.
+
+Fixpoint expression_traces e :=
+  match e with
+  | ⦃(_) = (_) ⊕[_] (_)⦄ => []
+  | ⦃if[b] (_) then {{e₀}} else {{e₁}}⦄ =>
+      (append_trace [(b, true)] (expression_traces e₀)) ++ (append_trace [(b, false)] (expression_traces e₁))
+  | ⦃{e₀}; {e₁}⦄ => append_trace_lists (expression_traces e₀) (expression_traces e₁)
+  end.
+
+Definition program_traces (p : program) :=
+  expression_traces (body p).
+
+
+
+
+
